Stuff.lean
@@ -1,3 +1,1 @@
-import Stuff.normalizing_properly.category
-
-def main : IO Unit := return ()
+def hello := "world"
