Stuff/normalizing_properly/prod_coprod_adj.lean
@@ -1,0 +1,543 @@
+import Mathlib.Tactic.Have
+
+structure Cat : Type :=
+( name : String )
+deriving DecidableEq
+
+structure FuncVar (C D : Cat) : Type :=
+(name : String)
+deriving DecidableEq
+
+inductive Func : Cat → Cat → Type
+| id (C : Cat) : Func C C
+| comp' {C D E : Cat} : FuncVar C D → Func D E → Func C E
+deriving DecidableEq
+
+def FuncVar.toFunc {C D : Cat} (F : FuncVar C D) : Func C D :=
+Func.comp' F $ Func.id _
+
+def Func.comp : {C D E : Cat} → Func C D → Func D E → Func C E
+| _, _, _, Func.id _, G => G
+| _, _, _, Func.comp' F G, H => Func.comp' F (comp G H)
+
+structure FData : Type :=
+( rel {C D : Cat} : Func C D → Func C D → Prop )
+[ decidRel {C D : Cat} : DecidableRel (@rel C D) ]
+( refl {C D : Cat} (F : Func C D) : rel F F )
+( symm {C D : Cat} {F G : Func C D} : rel G F → rel F G )
+( trans {C D : Cat} {F G H : Func C D} : rel F G → rel G H → rel F H )
+( rel_comp {C D E : Cat} {F₁ F₂ : Func C D} {G₁ G₂ : Func D E} :
+  rel F₁ F₂ → rel G₁ G₂ → rel (F₁.comp G₁) (F₂.comp G₂) )
+( hasRAdj {C D : Cat} : Func C D → Prop )
+[ decidHasRAdj {C D : Cat} (F : Func C D): Decidable (hasRAdj F) ]
+( hasRAdjCompLeft {C D E : Cat} (F : Func C E) (G : Func C D) (H : Func D E) :
+  rel F (G.comp H) → hasRAdj F → hasRAdj G )
+( hasRAdjCompRight {C D E : Cat} (F : Func C E) (G : Func C D) (H : Func D E) :
+  rel F (G.comp H) → hasRAdj F → hasRAdj H )
+( hasLAdj {C D : Cat} : Func C D → Prop )
+[ decidHasLAdj {C D : Cat} (F : Func C D): Decidable (hasLAdj F) ]
+( hasLAdjCompLeft {C D E : Cat} (F : Func C E) (G : Func C D) (H : Func D E) :
+  rel F (G.comp H) → hasLAdj F → hasLAdj G )
+( hasLAdjCompRight {C D E : Cat} (F : Func C E) (G : Func C D) (H : Func D E) :
+  rel F (G.comp H) → hasLAdj F → hasLAdj H )
+
+attribute [instance] FData.decidRel FData.decidHasRAdj FData.decidHasLAdj
+
+def FuncVar.hasRAdj {C D : Cat} (d : FData) (F : FuncVar C D) : Prop :=
+d.hasRAdj F.toFunc
+
+instance {C D : Cat} (d : FData) (F : FuncVar C D) : Decidable (F.hasRAdj d) :=
+d.decidHasRAdj _
+
+def FuncVar.hasLAdj {C D : Cat} (d : FData) (F : FuncVar C D) : Prop :=
+d.hasLAdj F.toFunc
+
+instance {C D : Cat} (d : FData) (F : FuncVar C D) : Decidable (F.hasLAdj d) :=
+d.decidHasLAdj _
+
+inductive Obj (d : FData) : Cat → Type
+| Ovar : String → Obj d C
+| prod : Obj d C → Obj d C → Obj d C
+| coprod : Obj d C → Obj d C → Obj d C
+| app {C D : Cat} : FuncVar C D → Obj d C → Obj d D
+| rAdjApp {C D : Cat} (F : FuncVar C D) : F.hasRAdj d → Obj d D → Obj d C
+| lAdjApp {C D : Cat} (F : FuncVar C D) : F.hasLAdj d → Obj d D → Obj d C
+| top : Obj d C
+| bot : Obj d C
+deriving DecidableEq
+
+namespace Obj
+
+variable {d : FData}
+
+inductive syn : {C : Cat} → (X Y : Obj d C) → Type
+| var {X Y : Obj d C} : String → syn X Y
+| prod_mk {X Y Z : Obj d C} (f : syn X Y) (g : syn X Z) :
+  syn X (prod Y Z)
+| coprod_mk {X Y Z : Obj d C} (f : syn X Z) (g : syn Y Z) :
+  syn (coprod X Y) Z
+| top_mk (X : Obj d C) : syn X top
+| bot_mk (X : Obj d C) : syn bot X
+| fst {X Y : Obj d C} : syn (prod X Y) X
+| snd {X Y : Obj d C} : syn (prod X Y) Y
+| inl {X Y : Obj d C} : syn X (coprod X Y)
+| inr {X Y : Obj d C} : syn Y (coprod X Y)
+| map {X Y : Obj d C} (F : FuncVar C D) (f : syn X Y) : syn (app F X) (app F Y)
+| rAdjMap {C D : Cat} {X Y : Obj d D} (F : FuncVar C D) (hF : F.hasRAdj d) (f : syn X Y) :
+  syn (rAdjApp F hF X) (rAdjApp F hF Y)
+| counit {C D : Cat} {X : Obj d D} (F : FuncVar C D) (hF : F.hasRAdj d) :
+  syn (app F (rAdjApp F hF X)) X
+| restrict {C D : Cat} {X : Obj d C} {Y : Obj d D} {F : FuncVar C D} (hF : F.hasRAdj d)
+  (f : syn (app F X) Y) : syn X (rAdjApp F hF Y)
+| lAdjMap {C D : Cat} {X Y : Obj d D} (F : FuncVar C D) (hF : F.hasLAdj d) (f : syn X Y) :
+  syn (lAdjApp F hF X) (lAdjApp F hF Y)
+| unit {C D : Cat} {X : Obj d D} (F : FuncVar C D) (hF : F.hasLAdj d) :
+  syn X (app F (lAdjApp F hF X))
+| extend {C D : Cat} {X : Obj d D} {Y : Obj d C} {F : FuncVar C D} (hF : F.hasLAdj d)
+  (f : syn X (app F Y)) : syn (lAdjApp F hF X) Y
+| id (X : Obj d C) : syn X X
+| comp {X Y Z : Obj d C} : syn X Y → syn Y Z → syn X Z
+
+def expandProds : {C : Cat} → Obj d C → Obj d C
+| _, Ovar X => Ovar X
+| _, prod X Y => prod (expandProds X) (expandProds Y)
+| _, coprod X Y => coprod (expandProds X) (expandProds Y)
+| _, app F (prod X Y) =>
+  if F.hasLAdj d then
+    prod (expandProds (app F X)) (expandProds (app F Y))
+  else app F (expandProds (prod X Y))
+| _, app F top =>
+  if F.hasLAdj d then top else app F top
+| _, app F (coprod X Y) =>
+  if F.hasRAdj d then
+    coprod (expandProds (app F X)) (expandProds (app F Y))
+  else app F (expandProds (coprod X Y))
+| _, app F bot =>
+  if F.hasRAdj d then bot else app F bot
+| _, app F X => app F (expandProds X)
+| _, rAdjApp F hF X => rAdjApp F hF (expandProds X)
+| _, lAdjApp F hF X => lAdjApp F hF (expandProds X)
+| _, top => top
+| _, bot => bot
+
+-- def toFactorProds : {C : Cat} → {X Y : Obj d C} → syn X Y → syn (expandProds X) (expandProds Y)
+-- | _, _, _, syn.var X => syn.var X
+-- | _, _, _, syn.prod_mk f g =>
+--   by rw [expandProds]; exact syn.prod_mk (toFactorProds f) (toFactorProds g)
+-- | _, _, _, syn.coprod_mk f g =>
+--   by rw [expandProds]; exact syn.coprod_mk (toFactorProds f) (toFactorProds g)
+-- | _, _, _, syn.top_mk X => by rw [expandProds]; exact syn.top_mk _
+-- | _, _, _, syn.bot_mk X => by rw [expandProds]; exact syn.bot_mk _
+-- | _, _, _, syn.fst => by rw [expandProds]; exact syn.fst
+-- | _, _, _, syn.snd => by rw [expandProds]; exact syn.snd
+-- | _, _, _, syn.inl => by rw [expandProds]; exact syn.inl
+-- | _, _, _, syn.inr => by rw [expandProds]; exact syn.inr
+-- | _, _, _, syn.comp f g => syn.comp (toFactorProds f) (toFactorProds g)
+-- | _, _, _, syn.id _ => syn.id _
+-- | _, _, _, syn.lAdjMap F hF f => by rw [expandProds]; exact syn.lAdjMap F hF (toFactorProds f)
+-- | _, _, _, syn.extend hF f => by rw [expandProds]; exact syn.extend hF (toFactorProds f)
+
+inductive syn2'_var_aux : {C : Cat} → (X Y : Obj d C) → Type
+| var {X Y : Obj d C} : String → syn2'_var_aux X Y
+| comp_fst {X Y Z : Obj d C} : syn2'_var_aux X (prod Y Z) → syn2'_var_aux X Y
+| comp_snd {X Y Z : Obj d C} : syn2'_var_aux X (prod Y Z) → syn2'_var_aux X Z
+| inl_comp {X Y Z : Obj d C} : syn2'_var_aux (coprod X Y) Z → syn2'_var_aux X Z
+| inr_comp {X Y Z : Obj d C} : syn2'_var_aux (coprod X Y) Z → syn2'_var_aux Y Z
+| unit_comp {C D : Cat} {X : Obj d D} {Y : Obj d C} (F : FuncVar C D) (hF : F.hasLAdj d) :
+  syn2'_var_aux (lAdjApp F hF X) Y → syn2'_var_aux X (app F Y)
+| comp_counit {C D : Cat} {X : Obj d C} {Y : Obj d D} (F : FuncVar C D) (hF : F.hasRAdj d) :
+  syn2'_var_aux X (rAdjApp F hF Y) → syn2'_var_aux (app F X) Y
+| expand_prods {C : Cat} {X Y : Obj d C} : syn2'_var_aux X Y →
+  syn2'_var_aux (expandProds X) (expandProds Y)
+
+def syn2'_var_aux_to_var : {C : Cat} → {X Y : Obj d C} →
+  syn2'_var_aux X Y → (C : Cat) × (_ _ : Obj d C) × String
+| C, X, Y, syn2'_var_aux.var s => ⟨C, X, Y, s⟩
+| _, _, _, syn2'_var_aux.comp_fst f => syn2'_var_aux_to_var f
+| _, _, _, syn2'_var_aux.comp_snd f => syn2'_var_aux_to_var f
+| _, _, _, syn2'_var_aux.inl_comp f => syn2'_var_aux_to_var f
+| _, _, _, syn2'_var_aux.inr_comp f => syn2'_var_aux_to_var f
+| _, _, _, syn2'_var_aux.unit_comp _ _ f => syn2'_var_aux_to_var f
+| _, _, _, syn2'_var_aux.comp_counit _ _ f => syn2'_var_aux_to_var f
+| _, _, _, syn2'_var_aux.expand_prods f => syn2'_var_aux_to_var f
+
+instance syn2'_var_aux_DecidableEq : {C : Cat} → {X Y : Obj d C} →
+  DecidableEq (syn2'_var_aux X Y)
+| C, X, Y, syn2'_var_aux.var s, syn2'_var_aux.var t =>
+  if hst : s = t then isTrue (by rw [hst]) else isFalse (by intro h; injection h; contradiction)
+| C, X, Y, syn2'_var_aux.comp_fst f, syn2'_var_aux.comp_fst g =>
+  by letI := syn2'_var_aux_DecidableEq f g;elan
+
+  if hfg : f = g then isTrue (by rw [hfg]) else isFalse (by intro h; injection h; contradiction)
+
+
+
+
+inductive isnt_limity : {C : Cat} → (X : Obj d C) → Prop
+| Ovar {X : String} : isnt_limity (Ovar X)
+| coprod (X Y : Obj d C) : isnt_limity (coprod X Y)
+| app {C D : Cat} {X : Obj d C} {Y : Obj d D} (F : FuncVar C D) : isnt_limity (app F X)
+| lAdjApp {C D : Cat} {X : Obj d D} (F : FuncVar C D) (hF : F.hasLAdj d) :
+  isnt_limity (lAdjApp F hF X)
+| bot : isnt_limity bot
+
+inductive isnt_limit : {C : Cat} → (X : Obj d C) → Prop
+| Ovar {X : String} : isnt_limit (Ovar X)
+| coprod (X Y : Obj d C) : isnt_limit (coprod X Y)
+| app {C D : Cat} {X : Obj d C} {Y : Obj d D} (F : FuncVar C D) : isnt_limit (app F X)
+| lAdjApp {C D : Cat} {X : Obj d D} (F : FuncVar C D) (hF : F.hasLAdj d) :
+  isnt_limit (lAdjApp F hF X)
+| rAdjApp {C D : Cat} {X : Obj d D} (F : FuncVar C D) (hF : F.hasRAdj d) :
+  isnt_limit (rAdjApp F hF X)
+| bot : isnt_limit bot
+
+inductive isnt_colimity : {C : Cat} → (X : Obj d C) → Prop
+| Ovar {X : String} : isnt_colimity (Ovar X)
+| prod (X Y : Obj d C) : isnt_colimity (prod X Y)
+| app {C D : Cat} {X : Obj d C} {Y : Obj d D} (F : FuncVar C D) : isnt_colimity (app F X)
+| rAdjApp {C D : Cat} {X : Obj d D} (F : FuncVar C D) (hF : F.hasRAdj d) :
+  isnt_colimity (rAdjApp F hF X)
+| top : isnt_colimity top
+
+
+inductive isnt_colimit : {C : Cat} → (X : Obj d C) → Prop
+| Ovar {X : String} : isnt_colimit (Ovar X)
+| prod (X Y : Obj d C) : isnt_colimit (prod X Y)
+| app {C D : Cat} {X : Obj d C} {Y : Obj d D} (F : FuncVar C D) : isnt_colimit (app F X)
+| rAdjApp {C D : Cat} {X : Obj d D} (F : FuncVar C D) (hF : F.hasRAdj d) :
+  isnt_colimit (rAdjApp F hF X)
+| lAdjApp {C D : Cat} {X : Obj d D} (F : FuncVar C D) (hF : F.hasLAdj d) :
+  isnt_colimit (lAdjApp F hF X)
+| top : isnt_colimit top
+
+inductive isExpanded : {C : Cat} → (X : Obj d C) → Prop
+| Ovar {X : String} : isExpanded (Ovar X)
+| prod (X Y : Obj d C) : isExpanded X → isExpanded Y → isExpanded (prod X Y)
+| coprod (X Y : Obj d C) : isExpanded X → isExpanded Y → isExpanded (coprod X Y)
+| top : isExpanded top
+| bot : isExpanded bot
+| rAdjApp {C D : Cat} {X : Obj d D} (F : FuncVar C D) (hF : F.hasRAdj d) : isExpanded X →
+  isExpanded (rAdjApp F hF X)
+| lAdjApp {C D : Cat} {X : Obj d D} (F : FuncVar C D) (hF : F.hasLAdj d) : isExpanded X →
+  isExpanded (lAdjApp F hF X)
+| appNotColimitNotLAdj {C D : Cat} {X : Obj d C} (F : FuncVar C D) : isnt_colimit X → ¬F.hasLAdj d →
+  isExpanded X → isExpanded (app F X)
+| appNotLimitNotRAdj {C D : Cat} {X : Obj d C} (F : FuncVar C D) : isnt_limit X → ¬F.hasRAdj d →
+  isExpanded X → isExpanded (app F X)
+| appNotLAdjNotRAdj {C D : Cat} {X : Obj d C} (F : FuncVar C D) : ¬F.hasLAdj d → ¬F.hasRAdj d →
+  isExpanded X → isExpanded (app F X)
+| appNotLimitNotColimit {C D : Cat} {X : Obj d C} (F : FuncVar C D) : isnt_limit X → isnt_colimit X →
+  isExpanded X → isExpanded (app F X)
+
+/-- No vars into prods, terminals or Radj, or out of coprods, initials or rAdjs. Every
+  var between prodFactors -/
+inductive syn2'_var : (X Y : Obj d C) → Type
+| mk_var {X Y : Obj d C} (hX : isnt_colimity X) (hY : isnt_limity Y) (hX' : isExpanded X) (hY' : isExpanded Y) :
+  syn2'_var_aux X Y → syn2'_var X Y
+
+#eval Lean.versionString
+
+mutual
+
+inductive syn2' : (X Y : Obj d C) → Type
+| var {X Y : Obj d C} : syn2'_var X Y → syn2' X Y
+| id (X : String) : syn2' (Ovar X) (Ovar X)
+| prod_mk {X Y Z : Obj d C} (f : syn2 X Y) (g : syn2 X Z) :
+  syn2' X (prod Y Z)
+| coprod_mk {X Y Z : Obj d C} (f : syn2 X Z) (g : syn2 Y Z) :
+  syn2' (coprod X Y) Z
+| extend {C D : Cat} {X : Obj d D} {Y : Obj d C} {F : FuncVar C D} (hF : F.hasLAdj d)
+  (f : syn2 X (app F Y)) : syn2' (lAdjApp F hF X) Y
+| restrict {C D : Cat} {X : Obj d C} {Y : Obj d D} {F : FuncVar C D} (hF : F.hasRAdj d)
+  (f : syn2 (app F X) Y) : syn2' X (rAdjApp F hF Y)
+| top_mk (X : Obj d C) : syn2' X top
+| bot_mk (X : Obj d C) : syn2' bot X
+| map {X Y : Obj d C} (F : FuncVar C D) (f : syn X Y) : syn2' (app F X) (app F Y)
+| fst_comp {X Y Z : Obj d C} (f : syn2 X Z) : syn2' (prod X Y) Z
+| snd_comp {X Y Z : Obj d C} (f : syn2 Y Z) : syn2' (prod X Y) Z
+| comp_inl {X Y Z : Obj d C} (f : syn2 X Y) : syn2' X (coprod Y Z)
+| comp_inr {X Y Z : Obj d C} (f : syn2 X Z) : syn2' X (coprod Y Z)
+| comp_unit {X Y : Obj d D} (F : FuncVar C D) (hF : F.hasLAdj d) (f : syn2 X Y) :
+  syn2' X (app F (lAdjApp F hF Y))
+| counit_comp {X Y : Obj d D} (F : FuncVar C D) (hF : F.hasRAdj d) (f : syn2 X Y) :
+  syn2' (app F (rAdjApp F hF X)) Y
+deriving DecidableEq
+
+inductive syn2 : (X Y : Obj d C) → Type
+| of' : {X Y : Obj d C} → syn2' X Y → syn2 X Y
+| comp' : {X Y Z : Obj d C} → syn2 X Y → syn2' Y Z → syn2 X Z
+
+end
+
+section decEq
+
+mutual
+
+def syn2'BEq : {X Y : Obj d C} → syn2' X Y → syn2' X Y → Bool
+| _, _, syn2'.var f, syn2'.var g => decide (f = g)
+| _, _, syn2'.id _, syn2'.id _ => true
+| _, _, syn2'.prod_mk f₁ g₁, syn2'.prod_mk f₂ g₂ =>
+  (syn2BEq f₁ f₂) && (syn2BEq g₁ g₂)
+| _, _, syn2'.coprod_mk f₁ g₁, syn2'.coprod_mk f₂ g₂ =>
+  (syn2BEq f₁ f₂) && (syn2BEq g₁ g₂)
+| _, _, @syn2'.top_mk _ _, @syn2'.top_mk _ _ => true
+| _, _, @syn2'.bot_mk _ _, @syn2'.bot_mk _ _ => true
+| _, _, syn2'.fst_comp f, syn2'.fst_comp g => syn2BEq f g
+| _, _, syn2'.snd_comp f, syn2'.snd_comp g => syn2BEq f g
+| _, _, syn2'.comp_inl f, syn2'.comp_inl g => syn2BEq f g
+| _, _, syn2'.comp_inr f, syn2'.comp_inr g => syn2BEq f g
+| _, _, _, _ => false
+
+def syn2BEq : {X Y : Obj d C} → syn2 X Y → syn2 X Y → Bool
+| _, _, syn2.of' f, syn2.of' g => syn2'BEq f g
+| _, _, @syn2.comp' _ _ Y₁ _ f₁ g₁, @syn2.comp' _ _ Y₂ _ f₂ g₂ =>
+  if hY : Y₁ = Y₂
+  then by subst hY; exact (syn2BEq f₁ f₂) && (syn2'BEq g₁ g₂)
+  else false
+| _, _, _, _ => false
+
+end
+
+axiom thing' {X Y : Obj d C}
+  {f g : syn2' X Y} : syn2'BEq f g = true ↔ f = g
+
+axiom thing {X Y : Obj d C}
+  {f g : syn2 X Y} : syn2BEq f g = true ↔ f = g
+
+instance {X Y : Obj d C} : DecidableEq (syn2' X Y) :=
+λ f g : syn2' X Y =>
+@decidable_of_decidable_of_iff (syn2'BEq f g = true) _ _ thing'
+
+instance {X Y : Obj d C} : DecidableEq (syn2 X Y) :=
+λ f g : syn2 X Y =>
+@decidable_of_decidable_of_iff (syn2BEq f g = true) _ _ thing
+
+end decEq
+
+namespace syn2
+
+def prod_mk {X Y Z : Obj d C}
+  (f : syn2 X Y) (g : syn2 X Z) : syn2 X (prod Y Z) :=
+syn2.of' (syn2'.prod_mk f g)
+
+def coprod_mk {X Y Z : Obj d C}
+  (f : syn2 X Z) (g : syn2 Y Z) : syn2 (coprod X Y) Z :=
+syn2.of' (syn2'.coprod_mk f g)
+
+def bot_mk (X : Obj d C) : syn2 bot X :=
+syn2.of' (syn2'.bot_mk X)
+
+def top_mk (X : Obj d C) : syn2 X top :=
+syn2.of' (syn2'.top_mk X)
+
+def fst_comp {X Y Z : Obj d C} (f : syn2 X Z) : syn2 (prod X Y) Z :=
+syn2.of' (syn2'.fst_comp f)
+
+def snd_comp {X Y Z : Obj d C} (f : syn2 Y Z) : syn2 (prod X Y) Z :=
+syn2.of' (syn2'.snd_comp f)
+
+def comp_inl {X Y Z : Obj d C} (f : syn2 X Y) : syn2 X (coprod Y Z) :=
+syn2.of' (syn2'.comp_inl f)
+
+def comp_inr {X Y Z : Obj d C} (f : syn2 X Z) : syn2 X (coprod Y Z) :=
+syn2.of' (syn2'.comp_inr f)
+
+def comp : {X Y Z : Obj d C} → syn2 X Y → syn2 Y Z → syn2 X Z
+| _, _, _, f, syn2.of' g => syn2.comp' f g
+| _, _, _, f, syn2.comp' g h => syn2.comp' (comp f g) h
+
+def id : {X : Obj d C} → syn2 X X
+| Ovar X => syn2.of' (syn2'.id X)
+| prod _ _ => syn2.prod_mk (syn2.fst_comp id) (syn2.snd_comp id)
+| coprod _ _ => syn2.coprod_mk (syn2.comp_inl id) (syn2.comp_inr id)
+| top => top_mk _
+| bot => bot_mk _
+
+def fst {X Y : Obj d C} : syn2 (prod X Y) X :=
+syn2.fst_comp syn2.id
+
+def snd {X Y : Obj d C} : syn2 (prod X Y) Y :=
+syn2.snd_comp syn2.id
+
+def inl {X Y : Obj d C} : syn2 X (coprod X Y) :=
+syn2.comp_inl syn2.id
+
+def inr {X Y : Obj d C} : syn2 Y (coprod X Y) :=
+syn2.comp_inr syn2.id
+
+unsafe def of_syn2'_var_aux : {X Y : Obj d C} → syn2'_var_aux X Y → syn2 X Y
+| Ovar _, Ovar _, v => syn2.of' $ syn2'.var (syn2'_var.Ovar_Ovar v)
+| Ovar _, coprod _ _, v => syn2.of' $ syn2'.var $ syn2'_var.Ovar_coprod v
+| Ovar _, bot, v => syn2.of' $ syn2'.var $ syn2'_var.Ovar_bot v
+| prod _ _, Ovar _, v => syn2.of' $ syn2'.var $ syn2'_var.prod_Ovar v
+| prod _ _, coprod _ _, v => syn2.of' $ syn2'.var $ syn2'_var.prod_coprod v
+| prod _ _, bot, v => syn2.of' $ syn2'.var $ syn2'_var.prod_bot v
+| top, Ovar _, v => syn2.of' $ syn2'.var $ syn2'_var.top_Ovar v
+| top, coprod _ _, v => syn2.of' $ syn2'.var $ syn2'_var.top_coprod v
+| top, bot, v => syn2.of' $ syn2'.var $ syn2'_var.top_bot v
+| _, top, _ => top_mk _
+| bot, _, _ => bot_mk _
+| _, prod _ _, v => prod_mk (of_syn2'_var_aux v.comp_fst) (of_syn2'_var_aux v.comp_snd)
+| coprod _ _, _, v => coprod_mk (of_syn2'_var_aux v.inl_comp) (of_syn2'_var_aux v.inr_comp)
+
+unsafe def var {X Y : Obj d C} (f : String) : syn2 X Y :=
+of_syn2'_var_aux (syn2'_var_aux.var f)
+
+mutual
+
+unsafe def cutelim_single :
+  {X Y : Obj d C} → (f : syn2' X Y) →
+  syn2' X Y × Bool -- Boolean indicates if any rewrites applied
+| _, _, syn2'.prod_mk f g =>
+  match cutelim f, cutelim g with
+  | ⟨f, b₁⟩, ⟨g, b₂⟩ => ⟨syn2'.prod_mk f g, b₁ || b₂⟩
+| _, _, syn2'.coprod_mk f g =>
+  match cutelim f, cutelim g with
+  | ⟨f, b₁⟩, ⟨g, b₂⟩ => ⟨syn2'.coprod_mk f g, b₁ || b₂⟩
+| _, _, f => ⟨f, false⟩
+
+/-- eliminates cuts from f ∘ g assuming f and g are both cut eliminated. -/
+unsafe def cutelim_pair :
+  {X Y Z : Obj d C} → (f : syn2' X Y) → (g : syn2' Y Z) →
+  syn2 X Z × Bool -- Boolean indicates if any rewrites applied
+| _, _, top, _, _ => ⟨syn2.top_mk _, true⟩
+| bot, _, _, _, _ => ⟨syn2.bot_mk _, true⟩
+| _, _, _, syn2'.prod_mk f _, syn2'.fst_comp g => ⟨(cutelim (f.comp g)).1, true⟩
+| _, _, _, syn2'.prod_mk _ f, syn2'.snd_comp g => ⟨(cutelim (f.comp g)).1, true⟩
+| _, _, _, syn2'.comp_inl f, syn2'.coprod_mk g _ => ⟨(cutelim (f.comp g)).1, true⟩
+| _, _, _, syn2'.comp_inr f, syn2'.coprod_mk _ g => ⟨(cutelim (f.comp g)).1, true⟩
+| _, _, _, f, syn2'.prod_mk g h =>
+  ⟨syn2.prod_mk (cutelim ((syn2.of' f).comp g)).1
+                (cutelim ((syn2.of' f).comp h)).1,
+  true⟩
+| _, _, _, syn2'.coprod_mk f g, h =>
+  ⟨syn2.coprod_mk (cutelim (f.comp' h)).1 (cutelim (g.comp' h)).1,
+    true⟩
+| _, _, _, f, syn2'.comp_inl g => ((cutelim (syn2.comp (syn2.of' f) g)).1.comp_inl, true)
+| _, _, _, f, syn2'.comp_inr g => ((cutelim (syn2.comp (syn2.of' f) g)).1.comp_inr, true)
+| _, _, _, syn2'.fst_comp f, g => ((cutelim (syn2.comp' f g)).1.fst_comp, true)
+| _, _, _, syn2'.snd_comp f, g => ((cutelim (syn2.comp' f g)).1.snd_comp, true)
+| _, _, _, syn2'.id _, g => (syn2.of' g, true)
+| _, _, _, f, syn2'.id _ => (syn2.of' f, true)
+| _, _, _, f, g => ⟨syn2.comp' (syn2.of' f) g, false⟩
+
+unsafe def cutelim :
+  {X Y : Obj d C} → (f : syn2 X Y) → syn2 X Y × Bool
+| _, _, syn2.of' f =>
+  let f' := cutelim_single f
+  ⟨syn2.of' f'.1, f'.2⟩
+| _, _, syn2.comp' f g =>
+  match cutelim f, cutelim_single g with
+  | ⟨syn2.of' f, b₁⟩, ⟨g, b₂⟩ =>
+    match cutelim_pair f g with
+    | ⟨fg, b₃⟩ => ⟨fg, b₁ || b₂ || b₃⟩
+  | ⟨syn2.comp' e f, b₁⟩, ⟨g, b₂⟩ =>
+    match cutelim_pair f g with
+    | ⟨fg, true⟩ => ⟨(cutelim (e.comp fg)).1, true⟩
+    | ⟨fg, false⟩ => ⟨e.comp fg, b₁ || b₂⟩
+
+end
+
+mutual
+
+/- Normalizing cut eliminated terms. -/
+
+unsafe def normalize_single_ce :
+  {X Y : Obj d C} → (f : syn2' X Y) → syn2 X Y × Bool
+| coprod X Y, Z, syn2'.coprod_mk f g =>
+  match X, Y, Z, normalize_ce f, normalize_ce g with
+  | _, _, _, (@comp' _ _ _ Y₁ Z f₁ f₂, b₁), (@comp' _ _ _ Y₂ _ g₁ g₂, b₂) =>
+    if h : Y₁ = Y₂
+    then by
+      subst h
+      exact if f₂ = g₂
+        then ((normalize_ce ((syn2.coprod_mk f₁ g₁).comp' f₂)).1, true)
+        else (syn2.coprod_mk (comp' f₁ f₂) (comp' g₁ g₂), b₁ || b₂)
+    else (syn2.coprod_mk (comp' f₁ f₂) (comp' g₁ g₂), b₁ || b₂)
+  | _, _, _, (syn2.of' (syn2'.comp_inl f), _), (syn2.of' (syn2'.comp_inl g), _) =>
+     ((normalize_ce (syn2.coprod_mk f g)).1.comp_inl, true)
+   | _, _, _, (syn2.of' (syn2'.comp_inr f), _), (syn2.of' (syn2'.comp_inr g), _) =>
+     ((normalize_ce (syn2.coprod_mk f g)).1.comp_inr, true)
+  | _, _, _, (syn2.of' (syn2'.prod_mk f g), _), (syn2.of' (syn2'.prod_mk h i), _) =>
+    (syn2.prod_mk (normalize_ce (syn2.coprod_mk f h)).1 (normalize_ce (syn2.coprod_mk g i)).1, true)
+  | _, _, _, (f, b₁), (g, b₂) => (syn2.coprod_mk f g, b₁ || b₂)
+| _, _, syn2'.fst_comp f =>
+  match normalize_ce f with
+  | (syn2.of' (syn2'.prod_mk f g), _) => (syn2.prod_mk (syn2.fst_comp f) (syn2.fst_comp g), true)
+  | (syn2.of' (syn2'.comp_inl f), _) => (syn2.comp_inl (syn2.fst_comp f), true)
+  | (syn2.of' (syn2'.comp_inr f), _) => (syn2.comp_inr (syn2.fst_comp f), true)
+  | (e, b) => (e.fst_comp, b)
+| _, _, syn2'.snd_comp f =>
+  match normalize_ce f with
+  | (syn2.of' (syn2'.prod_mk f g), _) => (syn2.prod_mk (syn2.snd_comp f) (syn2.snd_comp g), true)
+  | (syn2.of' (syn2'.comp_inl f), _) => (syn2.comp_inl (syn2.snd_comp f), true)
+  | (syn2.of' (syn2'.comp_inr f), _) => (syn2.comp_inr (syn2.snd_comp f), true)
+  | (e, b) => (e.snd_comp, b)
+| _, _, syn2'.comp_inl f =>
+  match normalize_ce f with
+  | (f, b) => (f.comp_inl, b)
+| _, _, syn2'.comp_inr f =>
+  match normalize_ce f with
+  | (f, b) => (f.comp_inr, b)
+| _, _, syn2'.prod_mk f g =>
+  match normalize_ce f, normalize_ce g with
+  | (f, false), (g, false) => (syn2.prod_mk f g, false)
+  | (f, _), (g, _) => (syn2.prod_mk f g, true)
+| _, _, f => (syn2.of' f, false)
+
+/-- Normalizes a pair assuming both parts of the pair are normalized -/
+unsafe def normalize_pair_ce :
+  {X Y Z : Obj d C} → (f : syn2' X Y) →
+  (g : syn2' Y Z) → syn2 X Z × Bool
+| _, _, _, f, syn2'.prod_mk g h =>
+  ⟨syn2.prod_mk (normalize_ce ((syn2.of' f).comp g)).1 (normalize_ce ((syn2.of' f).comp h)).1, true⟩
+| _, _, _, f, syn2'.comp_inl g => ((normalize_ce (syn2.comp (syn2.of' f) g)).1.comp_inl, true)
+| _, _, _, f, syn2'.comp_inr g => ((normalize_ce (syn2.comp (syn2.of' f) g)).1.comp_inr, true)
+| _, _, _, syn2'.fst_comp f, g => ((normalize_ce (syn2.comp' f g)).1.fst_comp, true)
+| _, _, _, syn2'.snd_comp f, g => ((normalize_ce (syn2.comp' f g)).1.snd_comp, true)
+| _, _, _, f, g => ⟨syn2.comp' (syn2.of' f) g, false⟩
+
+unsafe def normalize_ce :
+  {X Y : Obj d C} → (f : syn2 X Y) → syn2 X Y × Bool
+| _, _, syn2.of' f => normalize_single_ce f
+| _, _, syn2.comp' f g =>
+  match normalize_single_ce g with
+  | (syn2.of' g, b₁) =>
+    match normalize_ce f with
+    | (syn2.of' f, b₂) =>
+      let n := normalize_pair_ce f g
+      (n.1, b₁ || b₂ || n.2)
+    | (syn2.comp' e f, b₂) =>
+      match normalize_pair_ce f g with
+      | ⟨fg, true⟩ => let n := normalize_ce (e.comp fg)
+        (n.1, b₁ || b₂ || n.2)
+      | ⟨fg, false⟩ => (e.comp fg, b₁ || b₂)
+  | (g, _) => ((normalize_ce (f.comp g)).1, true)
+
+end
+
+unsafe def normalize
+  {X Y : Obj d C} (s : syn2 X Y) : syn2 X Y :=
+(normalize_ce (cutelim s).1).1
+
+unsafe def of_syn : {X Y : Obj d C} → (f : syn X Y) → syn2 X Y
+| _, _, syn.var f => syn2.var f
+| _, _, syn.comp f g => comp (of_syn f) (of_syn g)
+| _, _, syn.id _ => syn2.id
+| _, _, syn.inr => syn2.inr
+| _, _, syn.inl => syn2.inl
+| _, _, syn.fst => syn2.fst
+| _, _, syn.snd => syn2.snd
+| _, _, syn.bot_mk _ => syn2.bot_mk _
+| _, _, syn.top_mk _ => syn2.top_mk _
+| _, _, syn.coprod_mk f g => syn2.coprod_mk (of_syn f) (of_syn g)
+| _, _, syn.prod_mk f g => syn2.prod_mk (of_syn f) (of_syn g)
+
+end syn2
+
+namespace syn
+
+unsafe def beq {X Y : Obj d C} (f g : syn X Y) : Bool :=
+decide (syn2.normalize (syn2.of_syn f) = syn2.normalize (syn2.of_syn g))
+
+end syn
