Stuff/normalizing_properly/tests/prod_coprod_vars2.lean
@@ -1,0 +1,109 @@
+import Stuff.normalizing_properly.prod_coprod_vars2
+
+open prod_coprod prod_coprod.syn
+
+def U : prod_coprod := Ovar "U"
+def V : prod_coprod := Ovar "V"
+def W : prod_coprod := Ovar "W"
+def X : prod_coprod := Ovar "X"
+def Y : prod_coprod := Ovar "Y"
+def Z : prod_coprod := Ovar "Z"
+
+def uu : syn U U := var "uu"
+def uv : syn U V := var "uv"
+def uw : syn U W := var "uw"
+def ux : syn U X := var "ux"
+def uy : syn U Y := var "uy"
+def uz : syn U Z := var "uz"
+
+def vu : syn V U := var "vu"
+def vv : syn V V := var "vv"
+def vw : syn V W := var "vw"
+def vx : syn V X := var "vx"
+def vy : syn V Y := var "vy"
+def vz : syn V Z := var "vz"
+
+def wu : syn W U := var "wu"
+def wv : syn W V := var "wv"
+def ww : syn W W := var "ww"
+def wx : syn W X := var "wx"
+def wy : syn W Y := var "wy"
+def wz : syn W Z := var "wz"
+
+def xu : syn X U := var "xu"
+def xv : syn X V := var "xv"
+def xw : syn X W := var "xw"
+def xx : syn X X := var "xx"
+def xy : syn X Y := var "xy"
+def xz : syn X Z := var "xz"
+
+def yu : syn Y U := var "yu"
+def yv : syn Y V := var "yv"
+def yw : syn Y W := var "yw"
+def yx : syn Y X := var "yx"
+def yy : syn Y Y := var "yy"
+def yz : syn Y Z := var "yz"
+
+def zu : syn Z U := var "zu"
+def zv : syn Z V := var "zv"
+def zw : syn Z W := var "zw"
+def zx : syn Z X := var "zx"
+def zy : syn Z Y := var "zy"
+def zz : syn Z Z := var "zz"
+
+def v1 : syn (prod X Y) (prod Y Z) := var "v1"
+
+def opObj : prod_coprod → prod_coprod
+| Ovar X => Ovar X
+| bot => top
+| top => bot
+| coprod X Y => prod (opObj X) (opObj Y)
+| prod X Y => coprod (opObj X) (opObj Y)
+
+def op : {X Y : prod_coprod} → syn X Y → syn (opObj Y) (opObj X)
+| _, _, syn.var f => syn.var f
+| _, _, syn.comp f g => syn.comp (op g) (op f)
+| _, _, syn.id _ => syn.id _
+| _, _, syn.inl => syn.fst
+| _, _, syn.inr => syn.snd
+| _, _, syn.fst => syn.inl
+| _, _, syn.snd => syn.inr
+| _, _, syn.bot_mk _ => syn.top_mk _
+| _, _, syn.top_mk _ => syn.bot_mk _
+| _, _, syn.prod_mk f g => syn.coprod_mk (op f) (op g)
+| _, _, syn.coprod_mk f g => syn.prod_mk (op f) (op g)
+
+unsafe def bopeq {X Y : prod_coprod} (f g : syn X Y) : Bool :=
+f.beq g && (op f).beq (op g)
+
+#eval bopeq
+  ((prod_mk uv uw).comp fst)
+  uv
+
+#eval bopeq
+  ((coprod_mk vu xu).comp ((prod_mk uv uw).comp (prod_mk (fst.comp vw) (snd.comp ww))))
+  (coprod_mk (prod_mk (vu.comp (uv.comp vw)) ((vu.comp uw).comp ww))
+            (prod_mk (xu.comp (uv.comp vw)) ((xu.comp uw).comp ww)))
+
+#eval bopeq v1 (prod_mk (comp (prod_mk (comp v1 fst) (comp v1 snd)) fst) (comp v1 snd))
+
+#eval bopeq
+  (comp inl ((coprod_mk vu xu).comp (((prod_mk uv uw).comp (prod_mk (fst.comp vw) (snd.comp ww))).comp snd)))
+  (comp (comp inl (coprod_mk (prod_mk (vu.comp (uv.comp vw)) ((vu.comp uw).comp ww))
+            (prod_mk (xu.comp (uv.comp vw)) ((xu.comp uw).comp ww)))) snd)
+
+#eval bopeq
+  (comp ((coprod_mk vu xu).comp ((prod_mk uv uw).comp (prod_mk (fst.comp vw) (snd.comp ww)))) fst)
+  (comp (coprod_mk (prod_mk (vu.comp (uv.comp vw)) ((vu.comp uw).comp ww))
+            (prod_mk (xu.comp (uv.comp vw)) ((xu.comp uw).comp ww))) fst)
+
+#eval bopeq
+  (comp ((coprod_mk vu xu).comp ((prod_mk uv uw).comp (prod_mk (fst.comp vw) (snd.comp ww)))) (@inr X _))
+  (coprod_mk (comp (prod_mk (vu.comp (uv.comp vw)) ((vu.comp uw).comp ww)) inr)
+            (comp (prod_mk (xu.comp (uv.comp vw)) ((xu.comp uw).comp ww)) inr))
+
+#eval
+  let p : syn top (coprod top X) := inl
+  beq
+    (coprod_mk p inr)
+    (syn.id (coprod top X))
