stuff.lean
@@ -1,6 +1,0 @@
-import Stuff.normalizing_properly.prod_coprod
-import Stuff.normalizing_properly.category
-import Stuff.normalizing_properly.free_category
-import Stuff.normalizing_properly.tests.prod_coprod
-
-def main : IO Unit := return ()
